Prove 'run_path_start_repeats_has_earlier_sfyzxnn'
That is, if a run path revisits the start, it must contain a south
south-facing step with y = 0 and non-negative x. The body of this proof
is similar to the old theorem ('run_path_xaxis_south_of_path_loops')
which is now proven as a consequence of this.

The reason for this reorganization is that the old theorem says
nothing about the relative order of the 'sfyzxnn' step, and the step
which revisits the start. In order to prove that the 'Endgame' has no
duplicates, we need to be sure that the 'sfyzxnn' step comes first.

AngelDevil/Runner.lean
@@ -1786,39 +1786,37 @@ lemma run_path_xaxis_west_has_earlier_xaxis_south (D : Devil) (p n : Nat) (hnice
     absurd Fin.le_iff_val_le_val.mp (find_first_is_first f ⟨i, lt_trans ilt' j'lt⟩ ⟨hinn, hiyz, hwest⟩); simp
     exact ilt'
 
--- If the run path loops, there is some step in the path on the
--- positive x-axis, facing south.
-lemma run_path_xaxis_south_of_path_loops (D : Devil) (p n : Nat) (hnice : nice D p) :
-  list_has_dupes (RunPath D p n) → ∃ rs ∈ (RunPath D p n),
-  0 ≤ rs.x ∧ rs.y = 0 ∧ rs.u = uvec_down := by
-  intro hdupes
-  let ⟨_, _, _, blt, _⟩ := hdupes
+abbrev south_facing_yz_xnn (rs : RunState) :=
+  0 ≤ rs.x ∧ rs.y = 0 ∧ rs.u = uvec_down
+
+-- If any step in the run path returns to the start, there must be
+-- some earlier south-facing step on the non-negative x-axis
+lemma run_path_start_repeats_has_earlier_sfyzxnn (D : Devil) (p n : Nat) (hnice : nice D p) :
+  ∀ i (ilt : i < (RunPath D p n).length), i ≠ 0 → (RunPath D p n)[i] = run_start →
+  ∃ j, ∃ (jlt : j < i), south_facing_yz_xnn ((RunPath D p n)[j]'(lt_trans jlt ilt)) := by
+  intro i ilt inz hTi
   let BL := make_block_list D p (n + 1)
   let L := (RunPath D p n).length
   let T := trace L run_start BL
+  -- Prove the run path and trace are equivalent
+  have htrace := run_path_eq_trace_of_nice D p n (n + 1) (by rw [Nat.add_one_sub_one]) hnice
   have Lpos : 0 < L :=
-    lt_of_le_of_lt (Nat.zero_le _) blt
+    lt_of_le_of_lt (Nat.zero_le _) ilt
   have hnnil : T ≠ [] := by
     apply List.ne_nil_of_length_pos
     rwa [trace_length]
-  let i := (find_first_dupe T hnnil).1
-  have ilt : i < T.length := Fin.prop _
-  have ilt' : i < L := by
-    unfold T at ilt
-    rwa [trace_length] at ilt
-  -- Get the equivalent trace
-  have htrace := run_path_eq_trace_of_nice D p n (n + 1) (by rw [Nat.add_one_sub_one]) hnice
+  have ilt' : i < T.length := by
+    unfold T
+    rwa [← htrace]
   have hvalid := run_start_valid_of_nice D p hnice (n + 1)
-  have hdupes' : list_has_dupes T := by rwa [htrace] at hdupes
+  --have hdupes' : list_has_dupes T := by rwa [htrace] at hdupes
   -- As previously proven, the first repeated state is 'run_start', so T[i] = run_start
-  have hTi : T[i] = run_start := trace_start_is_first_dupe L run_start BL hdupes' hvalid
-  have ipos : 0 < i := by
-    rcases first_dupe_is_dupe _ hdupes' with ⟨_, hlt, _⟩
-    exact lt_of_le_of_lt (Nat.zero_le _) hlt
-  have inz : i ≠ 0 := Nat.ne_zero_of_lt ipos
+  --have hTi : T[i] = run_start := trace_start_is_first_dupe L run_start BL hdupes' hvalid
+  have ipos : 0 < i := Nat.pos_of_ne_zero inz
   have iplt : i - 1 < L :=
-    lt_of_le_of_lt (Nat.sub_le _ _) ilt'
-  have := congrArg (undo_next_step BL) ((trace_getElem_recurrence' L run_start BL i ipos ilt') ▸ hTi)
+    lt_of_le_of_lt (Nat.sub_le _ _) ilt
+  rw [getElem_congr_coll htrace] at hTi
+  have := congrArg (undo_next_step BL) ((trace_getElem_recurrence' L run_start BL i ipos ilt) ▸ hTi)
   -- In order to use 'undo_next_step' we need to show that the
   -- wall next to T[i-1] is in-fact a wall.
   have hblocked : left_of_runner T[i - 1] ∈ BL :=
@@ -1844,8 +1842,8 @@ lemma run_path_xaxis_south_of_path_loops (D : Devil) (p n : Nat) (hnice : nice D
       unfold uvec_left; simp
     rcases run_path_xaxis_west_has_earlier_xaxis_south
       D p n hnice (i - 1) iplt ⟨hxnonneg, hyz, hwest⟩ with ⟨j, jlt, _⟩
-    have jlt' : j < L := lt_trans jlt iplt
-    use (RunPath D p n)[j], List.getElem_mem jlt'
+    have jlt' : j < i := lt_of_lt_of_le jlt (Nat.sub_le _ _)
+    use j, jlt'
   · -- If the path moved forward to return to 'run_start', it was
     -- previously south of the x-axis. That means we can use
     -- 'run_path_intersects_xaxis_of_south' to show that the path
@@ -1855,17 +1853,52 @@ lemma run_path_xaxis_south_of_path_loops (D : Devil) (p n : Nat) (hnice : nice D
       rw [getElem_congr_coll htrace, this]; simp
     rcases run_path_intersects_xaxis_of_south D p n hnice (i - 1) iplt hyneg with ⟨j, jlt, hxnonneg, hyz, hudir⟩
     have jlt' : j < L := lt_trans jlt iplt
+    have jlt'' := lt_of_lt_of_le jlt (Nat.sub_le _ _)
     rcases hudir with lhs | rhs
     · -- If the path was previously on the x-axis facing south, that closes the goal
-      use (RunPath D p n)[j], List.getElem_mem jlt'
+      exact ⟨j, jlt'', hxnonneg, hyz, lhs⟩
     · -- Otherwise we can find some earlier step on the path where
       -- the runner *was* on the x-axis facing south
       rcases run_path_xaxis_west_has_earlier_xaxis_south
         D p n hnice j jlt' ⟨hxnonneg, hyz, rhs⟩ with ⟨k, klt, _⟩
-      have klt' : k < L := lt_trans klt jlt'
-      use (RunPath D p n)[k], List.getElem_mem klt'
+      have klt' : k < i := lt_trans klt jlt''
+      use k, klt'
   · -- Lastly, if the path returned to 'run_start' by making a left turn
     -- it was previously west of the y-axis, which is impossible.
     unfold undo_turn_left run_start uvec_up at this; simp at this
     absurd run_path_x_nonneg D p n (RunPath D p n)[i - 1] (List.getElem_mem iplt); push_neg
     rw [getElem_congr_coll htrace, this]; simp
+
+-- If the run path loops, there is some step in the path on the
+-- positive x-axis, facing south. Note that this theorem only
+-- states that such a cell exists. It says nothing about the
+-- relative order of the duplicate and sfyzxnn cell
+-- (for that we need the previous theorem)
+lemma run_path_xaxis_south_of_path_loops (D : Devil) (p n : Nat) (hnice : nice D p) :
+  list_has_dupes (RunPath D p n) → ∃ rs ∈ (RunPath D p n), south_facing_yz_xnn rs := by
+  intro hdupes
+  let BL := make_block_list D p (n + 1)
+  let L := (RunPath D p n).length
+  let T := trace L run_start BL
+  have Lpos : 0 < L := run_path_length_pos D p n
+  have hnnil : T ≠ [] := by
+    apply List.ne_nil_of_length_pos
+    rwa [trace_length]
+  -- Prove the run path and trace are equivalent
+  have htrace := run_path_eq_trace_of_nice D p n (n + 1) (by rw [Nat.add_one_sub_one]) hnice
+  have hvalid := run_start_valid_of_nice D p hnice (n + 1)
+  let i := (find_first_dupe T hnnil).1
+  have ilt : i < T.length := Fin.prop _
+  have ilt' : i < L := by rwa [trace_length] at ilt
+  have hdupes' : list_has_dupes T := by
+    unfold T
+    rwa [← htrace]
+  have hTi : T[i] = run_start := trace_start_is_first_dupe L run_start BL hdupes' hvalid
+  let ⟨_, lbi, _⟩ := first_dupe_is_dupe T hdupes'
+  have inz : i ≠ 0 := Nat.ne_zero_of_lt lbi
+  have hTi' : (RunPath D p n)[i] = run_start := by
+    rwa [getElem_congr_coll htrace]
+  -- Use our previous result to find the location of an 'sfyzxnn' step
+  rcases run_path_start_repeats_has_earlier_sfyzxnn D p n hnice i ilt' inz hTi' with ⟨j, jlt, _⟩
+  have jlt' : j < L := lt_trans jlt ilt'
+  use (RunPath D p n)[j], List.getElem_mem jlt'
